`as_f` and `as_validator` type checks

src/3d/prelude/EverParse3d.Actions.Base.fsti
@@ -152,14 +152,14 @@ val validate_with_action_t
       (#wk: _)
       (#k:parser_kind nz wk)
       (#t:Type)
-      (#ret:Type0) //return type of the validator
+      (#ret_t:Type0) //return type of the validator
       (p:parser k t)
       (liveness_inv:slice_inv)
       (disj:disjointness_pre)
       (l:eloc)
       (has_action:bool)
       (allow_reading:bool)
-      (f:t -> GTot ret) //ghost function that specifies which (subset of) parsed values are returned by the validator
+      (f:t -> GTot ret_t) //ghost function that specifies which (subset of) parsed values are returned by the validator
     : Type0
 
 inline_for_extraction noextract
@@ -173,8 +173,8 @@ val validate_eta
       (#[@@@erasable] disj:disjointness_pre)
       (#[@@@erasable] l:eloc)
       (#has_action #allow_reading:bool)
-      (#ret:Type0)
-      (#f:t -> GTot ret)
+      (#ret_t:Type0)
+      (#f:t -> GTot ret_t)
       (v: validate_with_action_t p inv disj l has_action allow_reading f)
 : Tot (validate_with_action_t p inv disj l has_action allow_reading f)
 
@@ -208,8 +208,8 @@ val validate_without_reading
       (#[@@@erasable] disj:disjointness_pre)
       (#[@@@erasable] l:eloc)
       (#has_action #allow_reading:bool)
-      (#ret: Type0)
-      (#f:t -> GTot ret)
+      (#ret_t: Type0)
+      (#f:t -> GTot ret_t)
       (v: validate_with_action_t p inv disj l has_action allow_reading f)
 : Tot (validate_with_action_t p inv disj l has_action false f)
 
@@ -225,8 +225,8 @@ val validate_with_success_action
       (#[@@@erasable] disj1:disjointness_pre)
       (#[@@@erasable] l1:eloc)
       (#has_action #allow_reading:bool)
-      (#ret: Type0)
-      (#f:t1 -> GTot ret)
+      (#ret_t: Type0)
+      (#f:t1 -> GTot ret_t)
       (v1:validate_with_action_t p1 inv1 disj1 l1 has_action allow_reading f)
       (#[@@@erasable] inv2:slice_inv)
       (#[@@@erasable] disj2:disjointness_pre)
@@ -248,14 +248,26 @@ val validate_with_error_handler
       (#[@@@erasable] disj:disjointness_pre)
       (#[@@@erasable] l1:eloc)
       (#has_action #ar:_)
-      (#ret: Type0)
-      (#f:t1 -> GTot ret)
+      (#ret_t: Type0)
+      (#f:t1 -> GTot ret_t)
       (v1:validate_with_action_t p1 inv1 disj l1 has_action ar f)
   : validate_with_action_t p1 inv1 disj l1 has_action ar f
 
+// fun _ -> ()
+let validate_ret_f (t) (x:t) : GTot unit = ()
+
 inline_for_extraction noextract
 val validate_ret
-  : validate_with_action_t (parse_ret ()) true_inv disjointness_trivial eloc_none false true (fun _ -> ())
+  : validate_with_action_t (parse_ret ()) true_inv disjointness_trivial eloc_none false true (validate_ret_f unit)
+
+// (fun (_, x2) -> f2 x2)
+let validate_pair_f 
+    (t1: Type)
+    (t2: Type)
+    (ret_t2: Type0)
+    (f2: t2 -> GTot ret_t2)
+    (x: (t1 & t2)) : GTot ret_t2 =
+    let (_, x2) = x in f2 x2 //nondep pair drops the first return value
 
 inline_for_extraction noextract
 val validate_pair
@@ -269,8 +281,8 @@ val validate_pair
        (#[@@@erasable] disj1:disjointness_pre)
        (#[@@@erasable] l1:eloc)
        (#has_action1 #allow_reading1:bool)
-       (#ret1: Type0)
-       (#f1: t1 -> GTot ret1)
+       (#ret_t1: Type0)
+       (#f1: t1 -> GTot ret_t1)
        (v1:validate_with_action_t p1 inv1 disj1 l1 has_action1 allow_reading1 f1)
        (#nz2:_)
        (#wk2: _)
@@ -282,8 +294,8 @@ val validate_pair
        (#[@@@erasable] disj2:disjointness_pre)
        (#[@@@erasable] l2:eloc)
        (#has_action2 #allow_reading2:bool)
-       (#ret2: Type0)
-       (#f2: t2 -> GTot ret2)
+       (#ret_t2: Type0)
+       (#f2: t2 -> GTot ret_t2)
        (v2:validate_with_action_t p2 inv2 disj2 l2 has_action2 allow_reading2 f2)
   : validate_with_action_t
       (p1 `parse_pair` p2)
@@ -292,7 +304,20 @@ val validate_pair
       (l1 `eloc_union` l2)
       (has_action1 || has_action2)
       false
-      (fun (_, x2) -> f2 x2)
+      (validate_pair_f t1 t2 ret_t2 f2)
+
+
+// (fun (| x1, x2 |) -> f2 (f1 x1) x2)
+let validate_dep_pair_gen_f 
+      (t1: Type)
+      (ret_t1: Type0)
+      (f1: t1 -> GTot ret_t1)
+      (t2: ret_t1 -> Type)
+      (ret_t2: Type0)
+      (f2: (x1:ret_t1) -> (x2: t2 x1) -> GTot ret_t2)
+      (x) : GTot ret_t2 =
+    let (|x1, x2|) = x in f2 (f1 x1) x2
+
 
 inline_for_extraction noextract
 val validate_dep_pair_gen 
@@ -305,21 +330,21 @@ val validate_dep_pair_gen
       (#[@@@erasable] disj1:disjointness_pre)
       (#[@@@erasable] l1:eloc)
       (#has_action1:_)
-      (#ret1: Type0)
-      (#f1: t1 -> GTot ret1)
-      (v1:validate_with_action_t p1 inv1 disj1 l1 has_action1 true f1)
+      (#ret_t1: Type0)
+      (#f1: t1 -> GTot ret_t1)
+      (v1:validate_with_action_t p1 inv1 disj1 l1 has_action1 false f1)
       (#nz2:_)
       (#wk2: _)
       (#k2:parser_kind nz2 wk2)
-      (#[@@@erasable] t2:ret1 -> Type)
-      (#[@@@erasable] p2:(x:ret1 -> parser k2 (t2 x)))
+      (#[@@@erasable] t2:ret_t1 -> Type)
+      (#[@@@erasable] p2:(x:ret_t1 -> parser k2 (t2 x)))
       (#[@@@erasable] inv2:slice_inv)
       (#[@@@erasable] disj2:disjointness_pre)
       (#[@@@erasable] l2:eloc)
       (#has_action2 #allow_reading2:bool)
-      (#ret2: Type0) //the return type of the second parser must not depend on the values read by the first parser (for extraction)
-      (#f2: (x1:ret1) -> (x2: t2 x1) -> GTot ret2)
-      (v2:(x: ret1 -> validate_with_action_t (p2 x) inv2 disj2 l2 has_action2 allow_reading2 (f2 x)))
+      (#ret_t2: Type0) //the return type of the second parser must not depend on the values read by the first parser (for extraction)
+      (#f2: (x1:ret_t1) -> (x2: t2 x1) -> GTot ret_t2)
+      (v2:(x: ret_t1 -> validate_with_action_t (p2 x) inv2 disj2 l2 has_action2 allow_reading2 (f2 x)))
   : validate_with_action_t
       (p1 `parse_dep_pair` (fun (x1:t1) -> p2 (f1 x1)))
       (conj_inv inv1 inv2)
@@ -327,7 +352,16 @@ val validate_dep_pair_gen
       (l1 `eloc_union` l2)
       (has_action1 || has_action2)
       false
-      (fun (| x1, x2 |) -> f2 (f1 x1) x2)
+      (validate_dep_pair_gen_f t1 ret_t1 f1 t2 ret_t2 f2)
+
+// (fun (| x1, x2 |) -> f2 x1 x2)
+let validate_dep_pair_f 
+      (t1: Type)
+      (t2: t1 -> Type)
+      (ret_t2: Type0)
+      (f2: (x1:t1) -> (x2: t2 x1) -> GTot ret_t2)
+      (x) : GTot ret_t2 =
+    let (|x1, x2|) = x in f2 x1 x2
 
 inline_for_extraction noextract
 val validate_dep_pair
@@ -340,7 +374,7 @@ val validate_dep_pair
       (#[@@@erasable] disj1:disjointness_pre)
       (#[@@@erasable] l1:eloc)
       (#has_action1:_)
-      (v1:validate_with_action_t p1 inv1 disj1 l1 has_action1 true (fun _ -> ()))
+      (v1:validate_with_action_t p1 inv1 disj1 l1 has_action1 true (validate_ret_f t1))
       (r1: leaf_reader p1)
       (#nz2:_)
       (#wk2: _)
@@ -351,8 +385,8 @@ val validate_dep_pair
       (#[@@@erasable] disj2:disjointness_pre)
       (#[@@@erasable] l2:eloc)
       (#has_action2 #allow_reading2:bool)
-      (#ret2: Type0) //the return type of the second parser must not depend on the values read by the first parser (for extraction)
-      (#f2: (x1:t1) -> (x2: t2 x1) -> GTot ret2)
+      (#ret_t2: Type0) //the return type of the second parser must not depend on the values read by the first parser (for extraction)
+      (#f2: (x1:t1) -> (x2: t2 x1) -> GTot ret_t2)
       (v2:(x:t1 -> validate_with_action_t (p2 x) inv2 disj2 l2 has_action2 allow_reading2 (f2 x)))
   : validate_with_action_t
       (p1 `parse_dep_pair` p2)
@@ -361,13 +395,35 @@ val validate_dep_pair
       (l1 `eloc_union` l2)
       (has_action1 || has_action2)
       false
-      (fun (| x1, x2 |) -> f2 x1 x2)
+      (validate_dep_pair_f t1 t2 ret_t2 f2)
+
+// (fun _ -> x)
+let validate_return_f 
+    (t:Type0)
+    (ret_t: Type0)
+    (x: ret_t) 
+    (a: t)
+    : GTot ret_t = 
+    x
 
 inline_for_extraction noextract
 val validate_return
-    (#t: Type0)
-    (x: t)
-  : validate_with_action_t (parse_ret ()) true_inv disjointness_trivial eloc_none false true (fun _ -> x)
+    (#ret_t: Type0)
+    (x: ret_t)
+  : validate_with_action_t (parse_ret ()) true_inv disjointness_trivial eloc_none false true (validate_return_f unit ret_t x)
+
+
+// (fun (| x1, x2 |) -> f2 x1 x2)
+let validate_dep_pair_with_refinement_and_action_gen_f
+      (t1: Type)
+      (ret_t1: Type0)
+      (f1: t1 -> GTot ret_t1)
+      (f: ret_t1 -> bool)
+      (t2:refine t1 (fun x1 -> f (f1 x1)) -> Type)
+      (ret_t2: Type0)
+      (f2: (x1:refine t1 (fun x1 -> f (f1 x1))) -> (x2: t2 x1) -> GTot ret_t2)
+      (x) : GTot ret_t2 =
+    let (|x1, x2|) = x in f2 x1 x2
 
 inline_for_extraction noextract
 val validate_dep_pair_with_refinement_and_action_gen
@@ -381,15 +437,15 @@ val validate_dep_pair_with_refinement_and_action_gen
       (#[@@@erasable] disj1:disjointness_pre)
       (#[@@@erasable] l1:eloc)
       (#has_action1:bool)
-      (#ret1: Type0)
-      (#f1: t1 -> Tot ret1) // TODO: cannot use GTot here, not sure if this can be erased
-      (v1:validate_with_action_t p1 inv1 disj1 l1 has_action1 true f1)
-      (f: ret1 -> bool)
+      (#ret_t1: Type0)
+      (#f1: t1 -> GTot ret_t1)
+      (v1:validate_with_action_t p1 inv1 disj1 l1 has_action1 false f1)
+      (f: ret_t1 -> bool)
       (#[@@@erasable] inv1':slice_inv)
       (#[@@@erasable] disj1':disjointness_pre)
       (#[@@@erasable] l1':eloc)
       (#b #rt:_)
-      (a:ret1 -> action inv1' disj1' l1' b rt bool)
+      (a:refine t1 (fun x1 -> f (f1 x1)) -> action inv1' disj1' l1' b rt bool)
       (#nz2:_)
       (#wk2: _)
       (#k2:parser_kind nz2 wk2)
@@ -399,8 +455,8 @@ val validate_dep_pair_with_refinement_and_action_gen
       (#[@@@erasable] disj2:disjointness_pre)
       (#[@@@erasable] l2:eloc)
       (#has_action2 #allow_reading2:bool)
-      (#ret2: Type0) //the return type of the second parser must not depend on the values read by the first parser (for extraction)
-      (#f2: (x1:refine t1 (fun x1 -> f (f1 x1))) -> (x2: t2 x1) -> GTot ret2)
+      (#ret_t2: Type0) //the return type of the second parser must not depend on the values read by the first parser (for extraction)
+      (#f2: (x1:refine t1 (fun x1 -> f (f1 x1))) -> (x2: t2 x1) -> GTot ret_t2)
       (v2:(x:refine t1 (fun x1 -> f (f1 x1)) -> validate_with_action_t (p2 x) inv2 disj2 l2 has_action2 allow_reading2 (f2 x)))
   : validate_with_action_t
       ((p1 `parse_filter` (fun (x1:t1) -> f (f1 x1))) `parse_dep_pair` p2)
@@ -409,7 +465,18 @@ val validate_dep_pair_with_refinement_and_action_gen
       (l1 `eloc_union` (l1' `eloc_union` l2))
       true
       false
-      (fun (| x1, x2 |) -> f2 x1 x2)
+      (validate_dep_pair_with_refinement_and_action_gen_f t1 ret_t1 f1 f t2 ret_t2 f2)
+
+
+// (fun (| x1, x2 |) -> f2 x1 x2)
+let validate_dep_pair_with_refinement_and_action_f
+      (t1: Type)
+      (f: t1 -> bool)
+      (t2: refine t1 f -> Type)
+      (ret_t2: Type0)
+      (f2: (x1:refine t1 f) -> (x2: t2 x1) -> GTot ret_t2)
+      (x) : GTot ret_t2 =
+    let (|x1, x2|) = x in f2 x1 x2
 
 inline_for_extraction noextract
 val validate_dep_pair_with_refinement_and_action
@@ -423,7 +490,7 @@ val validate_dep_pair_with_refinement_and_action
       (#[@@@erasable] disj1:disjointness_pre)
       (#[@@@erasable] l1:eloc)
       (#has_action1:bool)
-      (v1:validate_with_action_t p1 inv1 disj1 l1 has_action1 true (fun _ -> ()))
+      (v1:validate_with_action_t p1 inv1 disj1 l1 has_action1 true (validate_ret_f t1))
       (r1: leaf_reader p1)
       (f: t1 -> bool)
       (#[@@@erasable] inv1':slice_inv)
@@ -440,8 +507,8 @@ val validate_dep_pair_with_refinement_and_action
       (#[@@@erasable] disj2:disjointness_pre)
       (#[@@@erasable] l2:eloc)
       (#has_action2 #allow_reading2:bool)
-      (#ret2: Type0)
-      (#f2: (x1:refine _ f) -> (x2: t2 x1) -> GTot ret2)
+      (#ret_t2: Type0)
+      (#f2: (x1:refine _ f) -> (x2: t2 x1) -> GTot ret_t2)
       (v2:(x:refine _ f -> validate_with_action_t (p2 x) inv2 disj2 l2 has_action2 allow_reading2 (f2 x)))
   : validate_with_action_t
       ((p1 `parse_filter` f) `parse_dep_pair` p2)
@@ -450,7 +517,18 @@ val validate_dep_pair_with_refinement_and_action
       (l1 `eloc_union` (l1' `eloc_union` l2))
       true
       false
-      (fun (| x1, x2 |) -> f2 x1 x2)
+      (validate_dep_pair_with_refinement_and_action_f t1 f t2 ret_t2 f2)
+
+// (fun (| x1, x2 |) -> f2 (f1 x1) x2)
+let validate_dep_pair_with_action_gen_f
+      (t1: Type)
+      (ret_t1: Type0)
+      (f1: t1 -> GTot ret_t1)
+      (t2: ret_t1 -> Type)
+      (ret_t2: Type0)
+      (f2: (x1:ret_t1) -> (x2: t2 x1) -> GTot ret_t2)
+      (x) : GTot ret_t2 =
+    let (|x1, x2|) = x in f2 (f1 x1) x2
 
 inline_for_extraction noextract
 val validate_dep_pair_with_action_gen
@@ -462,26 +540,26 @@ val validate_dep_pair_with_action_gen
       (#[@@@erasable] disj1:disjointness_pre)
       (#[@@@erasable] l1:eloc)
       (#has_action1:_)
-      (#ret1: Type0)
-      (#f1: t1 -> GTot ret1)
-      (v1:validate_with_action_t p1 inv1 disj1 l1 has_action1 true f1)
+      (#ret_t1: Type0)
+      (#f1: t1 -> GTot ret_t1)
+      (v1:validate_with_action_t p1 inv1 disj1 l1 has_action1 false f1)
       (#[@@@erasable] inv1':slice_inv)
       (#[@@@erasable] disj1':disjointness_pre)
       (#[@@@erasable] l1':eloc)
       (#b #rt:_)
-      (a:ret1 -> action inv1' disj1' l1' b rt bool)
+      (a:ret_t1 -> action inv1' disj1' l1' b rt bool)
       (#nz2:_)
       (#wk2: _)
       (#k2:parser_kind nz2 wk2)
-      (#[@@@erasable] t2:ret1 -> Type)
-      (#[@@@erasable] p2:(x:ret1 -> parser k2 (t2 x)))
+      (#[@@@erasable] t2:ret_t1 -> Type)
+      (#[@@@erasable] p2:(x:ret_t1 -> parser k2 (t2 x)))
       (#[@@@erasable] inv2:slice_inv)
       (#[@@@erasable] disj2:disjointness_pre)
       (#[@@@erasable] l2:eloc)
       (#has_action2 #allow_reading2:_)
-      (#ret2: Type0)
-      (#f2: (x1:ret1) -> (x2: t2 x1) -> GTot ret2)
-      (v2:(x:ret1 -> validate_with_action_t (p2 x) inv2 disj2 l2 has_action2 allow_reading2 (f2 x)))
+      (#ret_t2: Type0)
+      (#f2: (x1:ret_t1) -> (x2: t2 x1) -> GTot ret_t2)
+      (v2:(x:ret_t1 -> validate_with_action_t (p2 x) inv2 disj2 l2 has_action2 allow_reading2 (f2 x)))
   : validate_with_action_t
       (p1 `(parse_dep_pair #nz1)` (fun (x1: t1) -> p2 (f1 x1)))
       (conj_inv inv1 (conj_inv inv1' inv2))
@@ -489,7 +567,7 @@ val validate_dep_pair_with_action_gen
       (l1 `eloc_union` (l1' `eloc_union` l2))
       true
       false
-      (fun (| x1, x2 |) -> f2 (f1 x1) x2)
+      (validate_dep_pair_with_action_gen_f t1 ret_t1 f1 t2 ret_t2 f2)
 
 inline_for_extraction noextract
 val validate_dep_pair_with_action
@@ -501,7 +579,7 @@ val validate_dep_pair_with_action
       (#[@@@erasable] disj1:disjointness_pre)
       (#[@@@erasable] l1:eloc)
       (#has_action1:_)
-      (v1:validate_with_action_t p1 inv1 disj1 l1 has_action1 true (fun _ -> ()))
+      (v1:validate_with_action_t p1 inv1 disj1 l1 has_action1 true (validate_ret_f t1))
       (r1: leaf_reader p1)
       (#[@@@erasable] inv1':slice_inv)
       (#[@@@erasable] disj1':disjointness_pre)
@@ -517,8 +595,8 @@ val validate_dep_pair_with_action
       (#[@@@erasable] disj2:disjointness_pre)
       (#[@@@erasable] l2:eloc)
       (#has_action2 #allow_reading2:_)
-      (#ret2: Type0)
-      (#f2: (x1:t1) -> (x2: t2 x1) -> GTot ret2)
+      (#ret_t2: Type0)
+      (#f2: (x1:t1) -> (x2: t2 x1) -> GTot ret_t2)
       (v2:(x:t1 -> validate_with_action_t (p2 x) inv2 disj2 l2 has_action2 allow_reading2 (f2 x)))
   : validate_with_action_t
       (p1 `(parse_dep_pair #nz1)` p2)
@@ -527,7 +605,7 @@ val validate_dep_pair_with_action
       (l1 `eloc_union` (l1' `eloc_union` l2))
       true
       false
-      (fun (| x1, x2 |) -> f2 x1 x2)
+      (validate_dep_pair_f t1 t2 ret_t2 f2)
 
 inline_for_extraction noextract
 val validate_dep_pair_with_refinement_gen
@@ -541,10 +619,10 @@ val validate_dep_pair_with_refinement_gen
       (#[@@@erasable] disj1:disjointness_pre)      
       (#[@@@erasable] l1:eloc)
       (#has_action1:_)
-      (#ret1: Type0)
-      (#f1: t1 -> Tot ret1)
-      (v1:validate_with_action_t p1 inv1 disj1 l1 has_action1 true f1)
-      (f: ret1 -> bool)
+      (#ret_t1: Type0)
+      (#f1: t1 -> GTot ret_t1)
+      (v1:validate_with_action_t p1 inv1 disj1 l1 has_action1 false f1)
+      (f: ret_t1 -> bool)
       (#nz2:_)
       (#wk2: _)
       (#k2:parser_kind nz2 wk2)
@@ -555,8 +633,8 @@ val validate_dep_pair_with_refinement_gen
       (#[@@@erasable] l2:eloc)
       (#allow_reading2:bool)
       (#has_action2:_)
-      (#ret2: Type0)
-      (#f2: (x1:refine t1 (fun x1 -> f (f1 x1))) -> (x2: t2 x1) -> GTot ret2)
+      (#ret_t2: Type0)
+      (#f2: (x1:refine t1 (fun x1 -> f (f1 x1))) -> (x2: t2 x1) -> GTot ret_t2)
       (v2:(x:refine t1 (fun x1 -> f (f1 x1)) -> validate_with_action_t (p2 x) inv2 disj2 l2 has_action2 allow_reading2 (f2 x)))
   : validate_with_action_t
       ((p1 `parse_filter` (fun x1 -> f (f1 x1))) `parse_dep_pair` p2)
@@ -565,7 +643,17 @@ val validate_dep_pair_with_refinement_gen
       (l1 `eloc_union` l2)
       (has_action1 || has_action2)
       false
-      (fun (| x1, x2 |) -> f2 x1 x2)
+      (validate_dep_pair_with_refinement_and_action_gen_f t1 ret_t1 f1 f t2 ret_t2 f2)
+
+// (fun (| x1, x2 |) -> f2 x1 x2)
+let validate_dep_pair_with_refinement_f
+      (t1: Type)
+      (f: t1 -> bool)
+      (t2: refine t1 f -> Type)
+      (ret_t2: Type0)
+      (f2: (x1:refine t1 f) -> (x2: t2 x1) -> GTot ret_t2)
+      (x) : GTot ret_t2 =
+    let (|x1, x2|) = x in f2 x1 x2
 
 inline_for_extraction noextract
 val validate_dep_pair_with_refinement
@@ -579,7 +667,7 @@ val validate_dep_pair_with_refinement
       (#[@@@erasable] disj1:disjointness_pre)      
       (#[@@@erasable] l1:eloc)
       (#has_action1:_)
-      (v1:validate_with_action_t p1 inv1 disj1 l1 has_action1 true (fun _ -> ()))
+      (v1:validate_with_action_t p1 inv1 disj1 l1 has_action1 true (validate_ret_f t1))
       (r1: leaf_reader p1)
       (f: t1 -> bool)
       (#nz2:_)
@@ -592,8 +680,8 @@ val validate_dep_pair_with_refinement
       (#[@@@erasable] l2:eloc)
       (#allow_reading2:bool)
       (#has_action2:_)
-      (#ret2: Type0)
-      (#f2: (x1:refine _ f) -> (x2: t2 x1) -> GTot ret2)
+      (#ret_t2: Type0)
+      (#f2: (x1:refine _ f) -> (x2: t2 x1) -> GTot ret_t2)
       (v2:(x:refine _ f -> validate_with_action_t (p2 x) inv2 disj2 l2 has_action2 allow_reading2 (f2 x)))
   : validate_with_action_t
       ((p1 `parse_filter` f) `parse_dep_pair` p2)
@@ -602,7 +690,15 @@ val validate_dep_pair_with_refinement
       (l1 `eloc_union` l2)
       (has_action1 || has_action2)
       false
-      (fun (| x1, x2 |) -> f2 x1 x2)
+      (validate_dep_pair_with_refinement_f t1 f t2 ret_t2 f2)
+
+let validate_filter_gen_f
+      (t: Type)
+      (ret_t: Type0)
+      (f: t -> GTot ret_t)
+      (pred:ret_t -> bool)
+      (x: refine t (fun x -> pred (f x))) : GTot ret_t = 
+      f x
 
 inline_for_extraction noextract
 val validate_filter_gen
@@ -615,13 +711,13 @@ val validate_filter_gen
        (#[@@@erasable] disj:disjointness_pre)                   
        (#[@@@erasable] l:eloc)
        (#has_action:_)
-       (#ret:Type0)
-       (#f:t -> Tot ret)
-       (v:validate_with_action_t p inv disj l has_action true f)
-       (pred:ret -> bool)
+       (#ret_t:Type0)
+       (#f:t -> GTot ret_t)
+       (v:validate_with_action_t p inv disj l has_action false f)
+       (pred:ret_t -> bool)
        (cr:string)
        (cf:string)
-  : validate_with_action_t (p `parse_filter` (fun x -> pred (f x))) inv disj l has_action false f
+  : validate_with_action_t (p `parse_filter` (fun x -> pred (f x))) inv disj l has_action false (validate_filter_gen_f t ret_t f pred)
 
 inline_for_extraction noextract
 val validate_filter
@@ -634,12 +730,13 @@ val validate_filter
        (#[@@@erasable] disj:disjointness_pre)                   
        (#[@@@erasable] l:eloc)
        (#has_action:_)
-       (v:validate_with_action_t p inv disj l has_action true (fun _ -> ()))
+       (v:validate_with_action_t p inv disj l has_action true (validate_ret_f t))
        (r:leaf_reader p)
        (f:t -> bool)
        (cr:string)
        (cf:string)
-  : validate_with_action_t (p `parse_filter` f) inv disj l has_action false (fun _ -> ())
+  : validate_with_action_t (p `parse_filter` f) inv disj l has_action false 
+      (validate_ret_f _)
 
 inline_for_extraction noextract
 val validate_filter_with_action_gen
@@ -652,17 +749,17 @@ val validate_filter_with_action_gen
        (#[@@@erasable] disj:disjointness_pre)                   
        (#[@@@erasable] l:eloc)
        (#has_action:_)
-       (#ret:Type0)
-       (#f:t -> Tot ret)
-       (v:validate_with_action_t p inv disj l has_action true f)
-       (pred:ret -> bool)
+       (#ret_t:Type0)
+       (#f:t -> GTot ret_t)
+       (v:validate_with_action_t p inv disj l has_action false f)
+       (pred:ret_t -> bool)
        (cr:string)
        (cf:string)
        (#b #rt:bool)
        (#[@@@erasable] inva:slice_inv)
        (#[@@@erasable] disja:disjointness_pre)                   
        (#[@@@erasable] la:eloc)
-       (a: ret -> action inva disja la b rt bool)
+       (a: ret_t -> action inva disja la b rt bool)
   : validate_with_action_t #nz
       (p `parse_filter` (fun x -> pred (f x)))
       (conj_inv inv inva)
@@ -670,7 +767,7 @@ val validate_filter_with_action_gen
       (eloc_union l la)
       true
       false
-      f
+      (validate_filter_gen_f t ret_t f pred)
 
 inline_for_extraction noextract
 val validate_filter_with_action
@@ -683,7 +780,7 @@ val validate_filter_with_action
        (#[@@@erasable] disj:disjointness_pre)                   
        (#[@@@erasable] l:eloc)
        (#has_action:_)
-       (v:validate_with_action_t p inv disj l has_action true (fun _ -> ()))
+       (v:validate_with_action_t p inv disj l has_action true (validate_ret_f t))
        (r:leaf_reader p)
        (f:t -> bool)
        (cr:string)
@@ -700,7 +797,7 @@ val validate_filter_with_action
       (eloc_union l la)
       true
       false
-      (fun _ -> ())
+      (validate_ret_f _)
 
 inline_for_extraction noextract
 val validate_with_dep_action_gen
@@ -713,14 +810,14 @@ val validate_with_dep_action_gen
        (#[@@@erasable] disj:disjointness_pre)                   
        (#[@@@erasable] l:eloc)
        (#has_action:_)
-       (#ret:Type0)
-       (#f:t -> Tot ret)
-       (v:validate_with_action_t p inv disj l has_action true f)
+       (#ret_t:Type0)
+       (#f:t -> GTot ret_t)
+       (v:validate_with_action_t p inv disj l has_action false f)
        (#b #rt:bool)
        (#[@@@erasable] inva:slice_inv)
        (#[@@@erasable] disja:disjointness_pre)                   
        (#[@@@erasable] la:eloc)
-       (a: ret -> action inva disja la b rt bool)
+       (a: ret_t -> action inva disja la b rt bool)
   : validate_with_action_t #nz
       p
       (conj_inv inv inva)
@@ -741,7 +838,7 @@ val validate_with_dep_action
        (#[@@@erasable] disj:disjointness_pre)                   
        (#[@@@erasable] l:eloc)
        (#has_action:_)
-       (v:validate_with_action_t p inv disj l has_action true (fun _ -> ()))
+       (v:validate_with_action_t p inv disj l has_action true (validate_ret_f t))
        (r:leaf_reader p)
        (#b #rt:bool)
        (#[@@@erasable] inva:slice_inv)
@@ -755,7 +852,7 @@ val validate_with_dep_action
       (eloc_union l la)
       true
       false
-      (fun _ -> ())
+      (validate_ret_f t)
 
 inline_for_extraction noextract
 val validate_weaken_left
@@ -769,8 +866,8 @@ val validate_weaken_left
        (#[@@@erasable] l:eloc)
        (#allow_reading:bool)
        (#has_action:_)
-       (#ret:Type0)
-       (#f:t -> Tot ret)
+       (#ret_t:Type0)
+       (#f:t -> GTot ret_t)
        (v:validate_with_action_t p inv disj l has_action allow_reading f)
        (#nz':_)
        (#wk': _)
@@ -789,8 +886,8 @@ val validate_weaken_right
        (#[@@@erasable] l:eloc)
        (#allow_reading:bool)
        (#has_action:_)
-       (#ret:Type0)
-       (#f:t -> Tot ret)
+       (#ret_t:Type0)
+       (#f:t -> GTot ret_t)
        (v:validate_with_action_t p inv disj l has_action allow_reading f)
        (#nz':_)
        (#wk': _)
@@ -800,7 +897,18 @@ val validate_weaken_right
 inline_for_extraction noextract
 val validate_impos
        (_:unit)
-  : validate_with_action_t (parse_impos ()) true_inv disjointness_trivial eloc_none false true (fun _ -> ())
+  : validate_with_action_t (parse_impos ()) true_inv disjointness_trivial eloc_none false true (validate_ret_f _)
+
+// (fun (x: t_ite e a b) -> if e then (f1()) x else (f2()) x)
+let validate_ite_f
+       (e:bool)
+       (ret_t:Type0)
+       ([@@@erasable] a:squash e -> Type)
+       ([@@@erasable] b:squash (not e) -> Type)
+       ([@@@erasable] f1:squash e -> a() -> GTot ret_t)
+       ([@@@erasable] f2:squash (not e) -> b() -> GTot ret_t)
+       (x: t_ite e a b) : GTot ret_t =
+  if e then (f1()) x else (f2()) x
 
 noextract inline_for_extraction
 val validate_ite
@@ -819,11 +927,11 @@ val validate_ite
        (#[@@@erasable] l2:eloc)
        (#ha2 #ar2:_)
        ([@@@erasable] p1:squash e -> parser k (a()))
-       (#ret:Type0) //the return type of both branches must be the same
-       (#f1:squash e -> a() -> GTot ret)
+       (#ret_t:Type0) //the return type of both branches must be the same
+       (#f1:squash e -> a() -> GTot ret_t)
        (v1:(squash e -> validate_with_action_t (p1()) inv1 disj1 l1 ha1 ar1 (f1())))
        ([@@@erasable] p2:squash (not e) -> parser k (b()))
-       (#f2:squash (not e) -> b() -> GTot ret)
+       (#f2:squash (not e) -> b() -> GTot ret_t)
        (v2:(squash (not e) -> validate_with_action_t (p2()) inv2 disj2 l2 ha2 ar2 (f2())))
   : validate_with_action_t
       (parse_ite e p1 p2)
@@ -832,7 +940,7 @@ val validate_ite
       (l1 `eloc_union` l2)
       (ha1 || ha2)
       false
-      (fun (x: t_ite e a b) -> if e then (f1()) x else (f2()) x)
+      (validate_ite_f e ret_t a b f1 f2)
 
 noextract inline_for_extraction
 val validate_nlist
@@ -846,10 +954,10 @@ val validate_nlist
        (#[@@@erasable] disj:disjointness_pre)                   
        (#[@@@erasable] l:eloc)
        (#ha #allow_reading:bool)
-       (#ret:Type0)
-       (#f:t -> GTot ret)
+       (#ret_t:Type0)
+       (#f:t -> GTot ret_t)
        (v: validate_with_action_t p inv disj l ha allow_reading f)
-: validate_with_action_t (parse_nlist n n_is_const p) inv disj l ha false (fun _ -> ()) // nlist validator does not return (would incur heap-allocation)
+: validate_with_action_t (parse_nlist n n_is_const p) inv disj l ha false (validate_ret_f _) // nlist validator does not return (would incur heap-allocation)
 
 noextract inline_for_extraction
 val validate_nlist_constant_size_without_actions
@@ -864,10 +972,10 @@ val validate_nlist_constant_size_without_actions
        (#[@@@erasable] disj:disjointness_pre)                   
        (#[@@@erasable] l:eloc)
        (#allow_reading:bool)
-       (#ret:Type0)
-       (#f:t -> GTot ret)
+       (#ret_t:Type0)
+       (#f:t -> GTot ret_t)
        (v: validate_with_action_t p inv disj l false allow_reading f)
-: Tot (validate_with_action_t (parse_nlist n n_is_const p) inv disj l false false (fun _ -> ())) // nlist validator does not return (would incur heap-allocation)
+: Tot (validate_with_action_t (parse_nlist n n_is_const p) inv disj l false false (validate_ret_f _)) // nlist validator does not return (would incur heap-allocation)
 
 noextract inline_for_extraction
 val validate_t_at_most
@@ -881,10 +989,10 @@ val validate_t_at_most
        (#[@@@erasable] disj:disjointness_pre)                   
        (#[@@@erasable] l:eloc)
        (#ha #ar:_)
-       (#ret:Type0)
-       (#f:t -> GTot ret)
+       (#ret_t:Type0)
+       (#f:t -> GTot ret_t)
        (v:validate_with_action_t p inv disj l ha ar f)
-  : Tot (validate_with_action_t (parse_t_at_most n p) inv disj l ha false (fun _ -> ())) // t_at_most validator does not return
+  : Tot (validate_with_action_t (parse_t_at_most n p) inv disj l ha false (validate_ret_f _)) // t_at_most validator does not return
 
 noextract inline_for_extraction
 val validate_t_exact
@@ -898,10 +1006,10 @@ val validate_t_exact
        (#[@@@erasable] disj:disjointness_pre)                   
        (#[@@@erasable] l:eloc)
        (#ha #ar:_)
-       (#ret:Type0)
-       (#f:t -> GTot ret)
+       (#ret_t:Type0)
+       (#f:t -> GTot ret_t)
        (v:validate_with_action_t p inv disj l ha ar f)
-  : Tot (validate_with_action_t (parse_t_exact n p) inv disj l ha false (fun _ -> ())) // t_exact validator does not return
+  : Tot (validate_with_action_t (parse_t_exact n p) inv disj l ha false (validate_ret_f _)) // t_exact validator does not return
 
 inline_for_extraction noextract
 val validate_with_comment
@@ -915,8 +1023,8 @@ val validate_with_comment
        (#[@@@erasable] disj:disjointness_pre)                   
        (#[@@@erasable] l:eloc)
        (#ha #allow_reading:bool)
-       (#ret:Type0)
-       (#f:t -> GTot ret)
+       (#ret_t:Type0)
+       (#f:t -> GTot ret_t)
        (v:validate_with_action_t p inv disj l ha allow_reading f)
   : validate_with_action_t p inv disj l ha allow_reading f
  
@@ -934,8 +1042,8 @@ val validate_weaken_inv_loc
        ([@@@erasable] inv':slice_inv{inv' `inv_implies` inv})
        ([@@@erasable] disj':disjointness_pre { disj' `imp_disjointness` disj })
        ([@@@erasable] l':eloc{l' `eloc_includes` l})
-       (#ret:Type0)
-       (#f:t -> GTot ret)
+       (#ret_t:Type0)
+       (#f:t -> GTot ret_t)
        (v:validate_with_action_t p inv disj l ha allow_reading f)
   : Tot (validate_with_action_t p inv' disj' l' ha allow_reading f)
 
@@ -954,17 +1062,17 @@ val read_impos
     : leaf_reader (parse_impos())
 
 inline_for_extraction
-let validator #nz #wk (#k:parser_kind nz wk) (#t:Type) (p:parser k t) (#ret:Type0) (f:t -> GTot ret)
+let validator #nz #wk (#k:parser_kind nz wk) (#t:Type) (p:parser k t) (#ret_t:Type0) (f:t -> GTot ret_t)
   = validate_with_action_t p true_inv disjointness_trivial eloc_none false true f
 
 inline_for_extraction
 let validator_maybe_action #nz #wk (#k:parser_kind nz wk) (#t:Type) (p:parser k t) (has_action:bool) 
-  (#ret:Type0) (f:t -> GTot ret)
+  (#ret_t:Type0) (f:t -> GTot ret_t)
   = validate_with_action_t p true_inv disjointness_trivial eloc_none has_action true f
 
 inline_for_extraction noextract
 val validate____UINT8
-  : validator parse____UINT8 (fun _ -> ())
+  : validator parse____UINT8 (validate_ret_f _)
 
 inline_for_extraction noextract
 val read____UINT8
@@ -972,7 +1080,7 @@ val read____UINT8
 
 inline_for_extraction noextract
 val validate____UINT8BE
-  : validator parse____UINT8BE (fun _ -> ())
+  : validator parse____UINT8BE (validate_ret_f _)
 
 inline_for_extraction noextract
 val read____UINT8BE
@@ -980,7 +1088,7 @@ val read____UINT8BE
 
 inline_for_extraction noextract
 val validate____UINT16BE
-  : validator parse____UINT16BE (fun _ -> ())
+  : validator parse____UINT16BE (validate_ret_f _)
 
 inline_for_extraction noextract
 val read____UINT16BE
@@ -988,7 +1096,7 @@ val read____UINT16BE
 
 inline_for_extraction noextract
 val validate____UINT32BE
-  : validator parse____UINT32BE (fun _ -> ())
+  : validator parse____UINT32BE (validate_ret_f _)
 
 inline_for_extraction noextract
 val read____UINT32BE
@@ -996,7 +1104,7 @@ val read____UINT32BE
 
 inline_for_extraction noextract
 val validate____UINT64BE
-  : validator parse____UINT64BE (fun _ -> ())
+  : validator parse____UINT64BE (validate_ret_f _)
 
 inline_for_extraction noextract
 val read____UINT64BE
@@ -1004,7 +1112,7 @@ val read____UINT64BE
 
 inline_for_extraction noextract
 val validate____UINT16
-  : validator parse____UINT16 (fun _ -> ())
+  : validator parse____UINT16 (validate_ret_f _)
 
 inline_for_extraction noextract
 val read____UINT16
@@ -1012,7 +1120,7 @@ val read____UINT16
 
 inline_for_extraction noextract
 val validate____UINT32
-  : validator parse____UINT32 (fun _ -> ())
+  : validator parse____UINT32 (validate_ret_f _)
 
 inline_for_extraction noextract
 val read____UINT32
@@ -1020,7 +1128,7 @@ val read____UINT32
 
 inline_for_extraction noextract
 val validate____UINT64
-  : validator parse____UINT64 (fun _ -> ())
+  : validator parse____UINT64 (validate_ret_f _)
 
 inline_for_extraction noextract
 val read____UINT64
@@ -1028,7 +1136,7 @@ val read____UINT64
 
 inline_for_extraction noextract
 val validate_unit
-  : validator parse_unit (fun _ -> ())
+  : validator parse_unit (validate_ret_f _)
 
 inline_for_extraction noextract
 val read_unit
@@ -1036,7 +1144,7 @@ val read_unit
 
 inline_for_extraction noextract
 val validate_unit_refinement (f:unit -> bool) (cf:string)
-  : validator (parse_unit `parse_filter` f) (fun _ -> ())
+  : validator (parse_unit `parse_filter` f) (validate_ret_f _)
 
 inline_for_extraction noextract
 val validate_string
@@ -1044,19 +1152,19 @@ val validate_string
        (#t: eqtype)
        (#[@@@erasable] p: parser k t)
        (#ha:_)
-       (v: validator_maybe_action p ha (fun _ -> ()))
+       (v: validator_maybe_action p ha (validate_ret_f _))
        (r: leaf_reader p)
        (terminator: t)
-  : Tot (validate_with_action_t (parse_string p terminator) true_inv disjointness_trivial eloc_none ha false (fun _ -> ()))
+  : Tot (validate_with_action_t (parse_string p terminator) true_inv disjointness_trivial eloc_none ha false (validate_ret_f _))
 
 inline_for_extraction noextract
 val validate_all_bytes
   : validate_with_action_t parse_all_bytes true_inv disjointness_trivial eloc_none false false // could be true
-    (fun _ -> ())
+    (validate_ret_f _)
 
 inline_for_extraction noextract
 val validate_all_zeros
-  : validate_with_action_t parse_all_zeros true_inv disjointness_trivial eloc_none false false (fun _ -> ())
+  : validate_with_action_t parse_all_zeros true_inv disjointness_trivial eloc_none false false (validate_ret_f _)
 
 ////////////////////////////////////////////////////////////////////////////////
 
@@ -1212,8 +1320,8 @@ val probe_then_validate
       (#ptr_t:Type0)
       (typename:string)
       (fieldname:string)
-      (#ret:Type0)
-      (#f:t -> GTot ret)
+      (#ret_t:Type0)
+      (#f:t -> GTot ret_t)
       (v:validate_with_action_t p inv disj l ha allow_reading f)
       (src:ptr_t)
       (as_u64: ptr_t -> PA.pure_external_action U64.t)
